Correctness heapify with alpha nodes

Projects/Lindmar_Joost/BinaryHeapTreeV.lean
@@ -65,16 +65,414 @@ def heapMin:  BinaryTree α → (α → ENat) → ENat
 def alphaMapMin (f: α → ENat) (a b: α): α  := if f a <=f b then a else b
 
 
-def treeMin:  BinaryTree α → (α → ENat) → Option α
-| leaf, _ => none
-| node l v r, f => alphaMapMin (λx: if x = some x' then f x' else ⊤) v (alphaMapMin f (treeMin l f) (treeMin r f))
+--def treeMin:  BinaryTree α → (α → ENat) → Option α
+--| leaf, _ => none
+--| node l v r, f => alphaMapMin (λx: if x = some x' then f x' else ⊤) v (alphaMapMin f (treeMin l f) (treeMin r f))
 
-lemma extractMinCorrectNode (bt l r: BinaryTree α) (v: α) (f: α → ENat): bt = node l v r  → isMinHeap bt f → ∃ bt', extractMin bt f = (some (treeMin bt f), bt') ∧ isMinHeap bt' f := by sorry
+-- lemma extractMinCorrectNode (bt l r: BinaryTree α) (v: α) (f: α → ENat): bt = node l v r  → isMinHeap bt f → ∃ bt', extractMin bt f = (some (treeMin bt f), bt') ∧ isMinHeap bt' f := by sorry
+def rootIsMinOfChildren: (BinaryTree α) → (α → ENat) →  Prop
+| leaf, _ => true
+| node l v r, f => match l, r with
+    | leaf, leaf => true
+    | leaf, node _ rv _ => f v <= f rv
+    | node _ lv _, leaf => f v <= f lv
+    | node _ lv _, node _ rv _ =>  f v <= f lv ∧ f v <= f rv
 
-def isEmpty (bt: BinaryTree ENat):= bt = leaf
+def isEmpty (bt: BinaryTree α):= bt = leaf
 
 def leftAndRightAreMinHeap: (BinaryTree α) →  (f: α → ENat) →  Prop
 | leaf, _ => true
 | node l _ r, f => isMinHeap l f ∧ isMinHeap r f
 
-lemma heapifyEstablishesMinHeap (bt: BinaryTree α) (f: α → ENat): (hbt: leftAndRightAreMinHeap bt f) → isMinHeap (heapify bt f) f := by sorry
+
+lemma minHeapThenLeftAndRightAreMinHeap (bt: BinaryTree α) (f: α → ENat): isMinHeap bt f → leftAndRightAreMinHeap bt f := by
+intro hbt
+fun_induction isMinHeap; all_goals (grind [leftAndRightAreMinHeap, isMinHeap])
+
+lemma minHeapThenRootIsMinOfChildren (bt: BinaryTree α) (f: α → ENat): isMinHeap bt f → rootIsMinOfChildren bt f := by
+intro hbt
+fun_induction isMinHeap; all_goals (grind [rootIsMinOfChildren])
+
+
+lemma leftAndRightAreMinHeapAndRootIsMinOfChildrenToMinHeap (bt: BinaryTree α) (f: α → ENat): leftAndRightAreMinHeap bt f ∧ rootIsMinOfChildren bt f → isMinHeap bt f := by
+intro hbt
+fun_induction isMinHeap; all_goals (simp [rootIsMinOfChildren, leftAndRightAreMinHeap] at hbt;simp[hbt])
+
+lemma leftAndRightAreMinHeapLeft (l: BinaryTree α) (r: BinaryTree α) (v: α) (f: α → ENat): leftAndRightAreMinHeap (node l v r) f → leftAndRightAreMinHeap l f := by
+intro hbt
+simp [leftAndRightAreMinHeap] at hbt
+simp [minHeapThenLeftAndRightAreMinHeap, hbt]
+
+
+lemma leftAndRightAreMinHeapRight (l: BinaryTree α) (r: BinaryTree α) (v: α) (f: α → ENat): leftAndRightAreMinHeap (node l v r) f → leftAndRightAreMinHeap r f := by
+intro hbt
+simp [leftAndRightAreMinHeap] at hbt
+simp [minHeapThenLeftAndRightAreMinHeap, hbt]
+
+lemma heapifyPreservesStructure (bt: BinaryTree α) (f: α → ENat): (∃ l r v, bt = node l v r) →  ∃ l' v' r', heapify bt f = node l' v' r' := by
+intro hbt
+fun_induction heapify; all_goals expose_names
+. obtain ⟨l, r, v, hbt⟩ := hbt
+  contradiction
+all_goals simp
+
+
+
+lemma heapifyPreservesStructureAndRootMin (bt: BinaryTree α) (f: α → ENat): (∃ l r v, bt = node l v r) →  ∃ l' v' r', heapify bt f = node l' v' r' ∧ f v' ≤ (heapMin bt f) := by
+intro hbt
+fun_induction heapify; all_goals expose_names
+. obtain ⟨l, r, v, hbt⟩ := hbt
+  contradiction
+all_goals grind [heapMin]
+
+def contains: (BinaryTree α) → α → Prop
+| leaf, _ => false
+| node l v r, v' => v=v' ∨ contains l v' ∨ contains r v'
+
+lemma heapifyPreservesMembers (bt: BinaryTree α) (v: α) (f: α → ENat): contains bt v → contains (heapify bt f) v := by
+intro hbt
+fun_induction heapify generalizing v; all_goals try grind[contains]
+
+lemma heapifyPreservesMembers2 (bt: BinaryTree α) (v: α) (f: α → ENat):  contains (heapify bt f) v → contains bt v := by
+intro hbt
+fun_induction heapify generalizing v; all_goals try grind[contains]
+
+lemma containsIsNode (bt: BinaryTree α) (v: α): contains bt v → ∃ l v' r, bt = node l v' r := by
+fun_induction contains; all_goals simp
+
+lemma minHeapRootMin (bt l r: BinaryTree α) (v: α) (f: α → ENat): bt = (node l v r) → isMinHeap bt f → f v = heapMin bt f := by
+intro hbt hmin
+fun_induction isMinHeap; all_goals grind [heapMin]
+
+lemma rootIsMinOfChildrenLeft (l r ll lr: BinaryTree α) (v lv: α) (f: α → ENat): rootIsMinOfChildren (node l v r) f →  l = (node ll lv lr) →  f v ≤ f lv := by
+  intros; expose_names
+  rw [h_1] at h
+  cases r; all_goals grind[rootIsMinOfChildren]
+
+
+lemma rootIsMinOfChildrenRight (l r rl rr: BinaryTree α) (v rv: α) (f: α → ENat): rootIsMinOfChildren (node l v r) f →  r = (node rl rv rr) → f v ≤ f rv := by
+  intros; expose_names
+  rw [h_1] at h
+  cases r; all_goals try grind[rootIsMinOfChildren]
+  . grind [rootIsMinOfChildren.eq_def]
+
+
+lemma minHeapMemberLeRoot (bt: BinaryTree α) (v: α) (f: α → ENat): isMinHeap bt f →  contains bt v →  heapMin bt f ≤ f v := by
+intro hmin hl
+fun_induction contains
+. contradiction
+. expose_names
+  cases hl; all_goals expose_names
+  . expose_names
+    rw [←h]
+    suffices f v = (l.node v r).heapMin f by grind
+    apply minHeapRootMin (l.node v r) l r v; all_goals grind
+  . cases h; all_goals expose_names
+    . have h2: l.contains v' := by exact h
+      apply containsIsNode at h2
+      obtain ⟨l'', v'', r'', h2 ⟩:= h2
+      have h3: l = l''.node v'' r'' := by exact h2
+      have hmin2: (l.node v r).isMinHeap f := by assumption
+      have hmin3: (l.node v r).isMinHeap f := by assumption
+      apply minHeapThenLeftAndRightAreMinHeap at hmin
+      simp [leftAndRightAreMinHeap] at hmin
+      have hlmin: l.isMinHeap f:= by grind
+      have hlmin2: l.isMinHeap f:= by grind
+      apply ih2 at hlmin
+      apply hlmin at h
+      grw[← h]
+      apply minHeapThenRootIsMinOfChildren at hmin2
+      apply rootIsMinOfChildrenLeft l r l'' r'' v v'' f hmin2 at h2
+      have hhl: f v'' = l.heapMin f:= by grind [minHeapRootMin]
+      have hh: f v = (l.node v r).heapMin f:= by grind [minHeapRootMin]
+      grw [← hh, ← hhl]
+      exact h2
+    . have h2: r.contains v' := by exact h
+      apply containsIsNode at h2
+      obtain ⟨l'', v'', r'', h2 ⟩:= h2
+      have h3: r = l''.node v'' r'' := by exact h2
+      have hmin2: (l.node v r).isMinHeap f:= by assumption
+      have hmin3: (l.node v r).isMinHeap f:= by assumption
+      apply minHeapThenLeftAndRightAreMinHeap at hmin
+      simp [leftAndRightAreMinHeap] at hmin
+      have hlmin: r.isMinHeap f:= by grind
+      have hlmin2: r.isMinHeap f:= by grind
+      apply ih1 at hlmin
+      apply hlmin at h
+      grw[← h]
+      apply minHeapThenRootIsMinOfChildren at hmin2
+      apply rootIsMinOfChildrenRight l r l'' r'' v v'' f hmin2 at h2
+      have hhl: f v'' = r.heapMin f:= by grind [minHeapRootMin]
+      have hh: f v = (l.node v r).heapMin f:= by grind [minHeapRootMin]
+      grw [← hh, ← hhl]
+      exact h2
+
+-- lemma heapifyEstablishesRootIsMinOfChildren (bt: BinaryTree α) (hbt: leftAndRightAreMinHeap bt): rootIsMinOfChildren (heapify bt f) := by
+-- fun_induction heapify; all_goals expose_names; all_goals try grind[rootIsMinOfChildren, leftAndRightAreMinHeap]
+-- .
+--  have hr: (rl.node rv rr).leftAndRightAreMinHeap := by
+--     grind [leftAndRightAreMinHeapRight]
+--   simp [leftAndRightAreMinHeap] at hr
+--   simp [leftAndRightAreMinHeap] at ih1
+--   obtain ⟨hr1, hr2⟩ := hr
+--   apply ih1 at hr1
+--   apply hr1 at hr2
+--   have: ∃ l' v' r', heapify (node rl v rr) = node l' v' r' := by
+--     simp [heapifyPreservesStructure (node rl v rr)]
+--   obtain ⟨rl', v', rr', hrw⟩ := this
+--   rw [hrw]
+--   simp[rootIsMinOfChildren]
+--   grw[h]
+--   rw [hrw] at hr2
+--   have: contains (node rl' v' rr') v := by
+--     rw [←hrw]
+--     apply heapifyPreservesMembers
+--     simp [contains]
+
+
+
+--   sorry
+-- all_goals sorry
+
+-- lemma heapifyEstablishesLeftAndRigthAreMinHeap (bt: BinaryTree α) (hbt: leftAndRightAreMinHeap bt): leftAndRightAreMinHeap (heapify bt f) := by
+-- fun_induction heapify; all_goals expose_names
+-- . simp [leftAndRightAreMinHeap]
+-- . simp [leftAndRightAreMinHeap, isMinHeap]
+-- . simp [leftAndRightAreMinHeap, isMinHeap]
+--   simp [leftAndRightAreMinHeap] at hbt
+--   have hbtr: (rl.node rv rr).leftAndRightAreMinHeap := by grind [←minHeapThenLeftAndRightAreMinHeap]
+--   apply ih1 at hbtr
+--   sorry
+-- all_goals sorry
+
+--lemma leftAndRightAreMinHeapAndRootIsMinImpliesIsHeap ()
+
+lemma heapifyPreservesMinHeap (bt: BinaryTree α) (f: α → ENat): isMinHeap bt f → bt = heapify bt f:= by
+fun_induction heapify; all_goals expose_names; all_goals try grind
+. intro hbt
+  by_contra
+  have hbtmin: f v = heapMin (leaf.node v (rl.node rv rr)) f:= by grind [minHeapRootMin]
+  grind[heapMin]
+. intro hbt
+  by_contra
+  have hbtmin: f v = heapMin ((ll.node lv lr).node v leaf) f:= by grind [minHeapRootMin]
+  grind[heapMin]
+. intro hbt
+  have hbtmin: f v = heapMin ((ll.node lv lr).node v (rl.node rv rr)) f:= by grind [minHeapRootMin]
+  grind[heapMin]
+. intro hbt
+  have hbtmin: f v = heapMin ((ll.node lv lr).node v (rl.node rv rr)) f:= by grind [minHeapRootMin]
+  grind[heapMin]
+
+lemma binTreeEqR (l r l' r': BinaryTree α) (v v': α): (node l v r) = (node l' v' r') → r = r' := by
+grind only
+
+lemma binTreeEqL (l r l' r': BinaryTree α) (v v': α): (node l v r) = (node l' v' r') → l = l' := by
+grind only
+
+-- lemma decreaseRootIsHeap (l r: BinaryTree α) (v v':  α): isMinHeap (node l v r) →  v' ≤ minHeap (node l v r) → isMinHeap (node l v' r) := by sorry
+
+lemma heapifyPreservesValues (tree r l: BinaryTree α) (v: α) (f: α → ENat): tree.heapify f = node r v l → contains tree v := by
+grind [contains, heapifyPreservesMembers2]
+
+lemma containsRootOrChildren (tree r l: BinaryTree α) (v v': α) : tree = node r v l → contains tree v' → contains r v' ∨ contains l v' ∨ v= v' := by
+grind [contains]
+
+
+lemma containsRootOrChildrenLeftLeaf (tree r: BinaryTree α) (v v':  α): tree = node r v leaf → contains tree v' → contains r v' ∨ v= v' := by
+grind [contains]
+
+lemma containsRightThenContainsRoot (tree l r: BinaryTree α) (v v':  α): tree = node l v r → contains r v' → contains tree v' := by
+grind [contains]
+
+lemma containsLeftThenContainsRoot (tree l r: BinaryTree α) (v v':  α): tree = node l v r → contains l v' → contains tree v' := by
+grind [contains]
+
+lemma heapifyEstablishesMinHeap' (bt l r: BinaryTree α) (v: α) (f: α → ENat): bt = node l v r ∧  isMinHeap l f ∧ isMinHeap r f → isMinHeap (heapify bt f) f := by
+fun_induction heapify generalizing l r v; all_goals expose_names
+. simp [isMinHeap]
+. simp [isMinHeap]
+. intro ⟨hr, hminl, hminr⟩
+  apply leftAndRightAreMinHeapAndRootIsMinOfChildrenToMinHeap
+  have: ∃ rl' v' rr', (rl.node v_1 rr).heapify f = node rl' v' rr' ∧ f v' ≤ heapMin (rl.node v_1 rr) f:= by
+        apply heapifyPreservesStructureAndRootMin
+        simp
+  obtain ⟨rl', v', rr', hr1, hr2⟩ := this
+  have hv: v=v_1 := by grind
+  have hrnode: r = (rl.node rv rr) := by
+        apply binTreeEqR at hr
+        simp [hr]
+  constructor
+  . simp [leftAndRightAreMinHeap]
+    constructor
+    . simp [isMinHeap]
+    . specialize ih1 rl rr v_1
+      simp at ih1
+      apply minHeapThenLeftAndRightAreMinHeap at hminr
+      simp [leftAndRightAreMinHeap] at hminr
+      simp [hrnode] at hminr
+      apply ih1; all_goals grind
+  . rw [hr1]
+    simp [rootIsMinOfChildren]
+    have hrvmin : f rv = heapMin (rl.node rv rr) f:= by
+      apply minHeapRootMin (rl.node rv rr) rl rr rv f (rfl)
+      rw[← hrnode]; exact hminr
+    have hcontains: contains (node rl v_1 rr) v' := by
+      apply heapifyPreservesMembers2
+      rw[hr1]
+      simp[contains]
+    have hcontains: contains (rl.node rv rr) v' ∨ v'= v_1 := by grind[contains]
+    cases hcontains
+    . expose_names
+      apply minHeapMemberLeRoot r v' at hminr
+      rw [← hrnode] at h_1
+      apply hminr at h_1
+      grw[← h_1]
+      rw[hrvmin]
+      rw[hrnode]
+    . expose_names
+      rw [h_1]
+      grw [h]
+. grind [isMinHeap]
+. intro ⟨hl, hminl, hminr⟩
+  apply leftAndRightAreMinHeapAndRootIsMinOfChildrenToMinHeap
+  have: ∃ ll' v' lr', (ll.node v_1 lr).heapify f = node ll' v' lr' ∧ f v' ≤ heapMin (ll.node v_1 lr) f:= by
+        apply heapifyPreservesStructureAndRootMin
+        simp
+  obtain ⟨rl', v', rr', hr1, hr2⟩ := this
+  have hv: v=v_1 := by grind
+  have hlnode: l = (ll.node lv lr) := by
+        apply binTreeEqL at hl
+        simp [hl]
+  constructor
+  . simp [leftAndRightAreMinHeap]
+    constructor
+    . specialize ih1 ll lr v_1
+      simp at ih1
+      apply minHeapThenLeftAndRightAreMinHeap at hminl
+      simp [leftAndRightAreMinHeap] at hminl
+      simp [hlnode] at hminl
+      apply ih1; all_goals grind
+    . simp [isMinHeap]
+  . rw [hr1]
+    simp [rootIsMinOfChildren]
+    have hlvmin : f lv = heapMin (ll.node lv lr) f:= by
+      apply minHeapRootMin (ll.node lv lr) ll lr lv f (rfl)
+      rw[← hlnode]; exact hminl
+    have hcontains: contains (node ll v_1 lr) v' := by
+      apply heapifyPreservesMembers2
+      rw[hr1]
+      simp[contains]
+    have hcontains: contains (ll.node lv lr) v' ∨ v'= v_1 := by grind[contains]
+    cases hcontains
+    . expose_names
+      apply minHeapMemberLeRoot l v' at hminl
+      rw [← hlnode] at h_1
+      apply hminl at h_1
+      grw[← h_1]
+      rw[hlvmin]
+      rw[hlnode]
+    . expose_names
+      rw [h_1]
+      grw [h]
+. grind [isMinHeap]
+. grind [isMinHeap]
+. intro ⟨hl, hminl, hminr⟩
+  apply leftAndRightAreMinHeapAndRootIsMinOfChildrenToMinHeap
+  have: ∃ ll' v' lr', (ll.node v_1 lr).heapify f = node ll' v' lr' ∧ f v' ≤ heapMin (ll.node v_1 lr) f:= by
+        apply heapifyPreservesStructureAndRootMin
+        simp
+  obtain ⟨rl', v', rr', hr1, hr2⟩ := this
+  have hv: v=v_1 := by grind
+  have hlnode: l = (ll.node lv lr) := by
+        apply binTreeEqL at hl
+        simp [hl]
+  constructor
+  . simp [leftAndRightAreMinHeap]
+    constructor
+    . specialize ih1 ll lr v_1
+      simp at ih1
+      apply minHeapThenLeftAndRightAreMinHeap at hminl
+      simp [leftAndRightAreMinHeap] at hminl
+      simp [hlnode] at hminl
+      apply ih1; all_goals grind
+    . grind
+  . rw [hr1]
+    simp [rootIsMinOfChildren]
+    have hlvmin : f lv = heapMin (ll.node lv lr) f := by
+      apply minHeapRootMin (ll.node lv lr) ll lr lv f (rfl)
+      rw[← hlnode]; exact hminl
+    have hcontains: contains (node ll v_1 lr) v' := by
+      apply heapifyPreservesMembers2
+      rw[hr1]
+      simp[contains]
+    have hcontains: contains (ll.node lv lr) v' ∨ v'= v_1 := by grind[contains]
+    cases hcontains
+    . expose_names
+      apply minHeapMemberLeRoot l v' at hminl
+      grind
+    . expose_names
+      grind
+. grind [isMinHeap]
+. intro ⟨hr, hminl, hminr⟩
+  apply leftAndRightAreMinHeapAndRootIsMinOfChildrenToMinHeap
+  have: ∃ rl' v' rr', (rl.node v_1 rr).heapify f = node rl' v' rr' ∧ f v' ≤ heapMin (rl.node v_1 rr) f:= by
+        apply heapifyPreservesStructureAndRootMin
+        simp
+  obtain ⟨rl', v', rr', hr1, hr2⟩ := this
+  have hv: v=v_1 := by grind
+  have hrnode: r = (rl.node rv rr) := by
+        apply binTreeEqR at hr
+        simp [hr]
+  constructor
+  . simp [leftAndRightAreMinHeap]
+    constructor
+    . grind
+    . specialize ih1 rl rr v_1
+      simp at ih1
+      apply minHeapThenLeftAndRightAreMinHeap at hminr
+      simp [leftAndRightAreMinHeap] at hminr
+      simp [hrnode] at hminr
+      apply ih1
+      . grind
+      . obtain ⟨h1, h2⟩ := hminr
+        exact h2
+  . rw [hr1]
+    simp [rootIsMinOfChildren]
+    have hrvmin : f rv = heapMin (rl.node rv rr) f := by
+      apply minHeapRootMin (rl.node rv rr) rl rr rv f (rfl)
+      rw[← hrnode]; exact hminr
+    have hcontains: contains (node rl v_1 rr) v' := by
+      apply heapifyPreservesMembers2
+      rw[hr1]
+      simp[contains]
+    have hcontains: contains (rl.node rv rr) v' ∨ v'= v_1 := by
+      apply containsRootOrChildren (node rl v_1 rr) rl rr v_1 v' (rfl) at hcontains
+      cases hcontains; all_goals expose_names
+      . left
+        apply containsLeftThenContainsRoot (node rl rv rr) rl rr rv v' (rfl) (h_2)
+      . cases h_2; all_goals expose_names
+        . left
+          apply containsRightThenContainsRoot (node rl rv rr) rl rr rv v' (rfl) (h_2)
+        . right
+          rw [h_2]
+    constructor
+    . simp at h
+      grw [h]
+    cases hcontains
+    . expose_names
+      apply minHeapMemberLeRoot r v' at hminr
+      rw [← hrnode] at h_2
+      apply hminr at h_2
+      grw[← h_2]
+      rw[hrvmin]
+      rw[hrnode]
+    . expose_names
+      rw [h_2]
+      simp at h_1
+      grw [h_1]
+
+lemma heapifyEstablishesMinHeap (bt: BinaryTree α) (f: α → ENat): (hbt: leftAndRightAreMinHeap bt f) → isMinHeap (heapify bt f) f := by
+cases bt
+. grind[isMinHeap,leftAndRightAreMinHeap, heapify]
+. grind[isMinHeap,leftAndRightAreMinHeap, heapifyEstablishesMinHeap']
